GradVer21Determ.v
@@ -1,0 +1,82 @@
+Load GradVer20Hook_import.
+Import Semantics.
+
+Definition inB {T:Type} (eq_dec : ∀ n m : T, {n = m} + {n ≠ m}) (x : T) (xs : list T) : bool :=
+  if in_dec eq_dec x xs
+  then true
+  else false.
+
+Lemma inB_In : forall {T:Type} ed (x : T) xs,
+  inB ed x xs = true <-> In x xs.
+Proof.
+  intros.
+  unfold inB.
+  destruct in_dec; cut.
+  split; cut.
+Qed.
+
+Definition evalphi'B (h : H) (r : rho) (a : A_d) (p : phi') : bool :=
+  match p with
+  | phiTrue => true
+  | phiEq e1 e2 => match evale' h r e1 with
+                   | None => false
+                   | Some v1 => 
+                     match evale' h r e2 with
+                     | None => false
+                     | Some v2 => v_decb v1 v2
+                     end
+                   end
+  | phiNeq e1 e2 =>match evale' h r e1 with
+                   | None => false
+                   | Some v1 => 
+                     match evale' h r e2 with
+                     | None => false
+                     | Some v2 => negb (v_decb v1 v2)
+                     end
+                   end
+  | phiAcc e f =>  match evale' h r e with
+                   | Some (vo o) => inB A'_d_dec (o, f) a
+                   | _ => false
+                   end
+  end.
+
+Lemma evalphi'B_works : forall h r a p,
+  evalphi'B h r a p = true <->
+  evalphi'  h r a p.
+Proof.
+  intros.
+  unfold evalphi'B.
+  destruct p0.
+  - split; cut.
+  - split; intros.
+    * destruct (evale' h r e) eqn: ev1; cut.
+      destruct (evale' h r e0) eqn: ev2; cut.
+      eca.
+      dec v_dec; cut.
+    * inv H.
+      rewrite H3, H7.
+      dec v_dec; auto.
+  - split; intros.
+    * destruct (evale' h r e) eqn: ev1; cut.
+      destruct (evale' h r e0) eqn: ev2; cut.
+      eca.
+      dec v_dec; cut.
+    * inv H.
+      rewrite H3, H7.
+      dec v_dec; auto.
+  - split; intros.
+    * destruct (evale' h r e) eqn: ev; cut.
+      destruct v; cut.
+      eca.
+      eapply inB_In; eauto.
+    * inv H.
+      rewrite H6.
+      apply inB_In.
+      auto.
+Qed.
+
+
+  
+  
+  
+  
